Diff/TraceModel.v
@@ -1,7 +1,6 @@
 From mathcomp Require Import all_ssreflect.
 
 Set Implicit Arguments.
-Unset Strict Implicit.
 Unset Printing Implicit Defensive. 
 
 Require Import ClassicalExtras.
@@ -9,73 +8,72 @@ Require Import Setoid.
 Require Import List.
 Require Import Stream.
 
-Record Events (event : Set) := {
+Record Events := {
 
-                  an_event : event;
-                  another_event : event;
-                  different_events : an_event <> another_event;
-                  eq_event_dec : forall (e1 e2 : event), {e1 = e2} + {e1 <> e2} 
+               event : Set;       
+               an_event : event;
+               another_event : event;
+               different_events : an_event <> another_event;
+               eq_event_dec : forall (e1 e2 : event), {e1 = e2} + {e1 <> e2} 
+               }. 
 
-                }. 
 
-Record EndState (endstate : Set) := { an_endstate : endstate }. 
+Record EndState := {
 
-Section Trace.
+              endstate : Set;            
+              an_endstate : endstate
+              }. 
 
-  Variable event : Set.
-  Variable endstate : Set.
-
-  Variable events : Events event. 
-  Variable endstates : EndState endstate.
-  
-  (** A trace represents either a stopped execution, a silently diverging
+(** A trace represents either a stopped execution, a silently diverging
     execution or an infinite execution. *)
-  Variant trace : Set :=
-  | tstop (l : list event) (e : endstate) : trace
-  | tsilent (l : list event) : trace
-  | tstream (s : @stream event) : trace.
+Variant trace {E : Events} {Es : EndState} : Set :=
+| tstop (l : list (event E)) (e : endstate Es) : trace
+| tsilent (l : list (event E)) : trace
+| tstream (s : @stream (event E)) : trace.
+
+
+Definition finite {E: Events} {Es : EndState} (t : @trace E Es) : Prop :=
+  exists l e, t = tstop l e.
+
+Definition infinite {E: Events} {Es : EndState} (t : @trace E Es) : Prop :=
+  ~ finite t. 
   
 
-  Definition finite (t : trace): Prop :=
-    exists l e, t = tstop l e.
-
-  Definition infinite (t : trace): Prop := ~ finite t. 
-  
-
-  (** A finite prefix is a list of events, that can be continued (ftbd)
+(** A finite prefix is a list of events, that can be continued (ftbd)
     or not (fstop). *)
-  Variant finpref : Set :=
-  | fstop (l : list event) (es : endstate) : finpref
-  | ftbd  (l : list event) : finpref. 
+Variant finpref {E : Events} {Es : EndState} : Set :=
+| fstop (l : list (event E)) (es : (endstate Es)) : finpref
+| ftbd  (l : list (event E)) : finpref. 
 
-  Tactic Notation "destruct" "finpref" ident(m) "as" ident(e) ident(f) ident(p) :=
-    destruct m as [ [| e p] f
-                  | [| e p]
-                  ].
+Tactic Notation "destruct" "finpref" ident(m) "as" ident(e) ident(f) ident(p) :=
+  destruct m as [ [| e p] f
+                | [| e p]
+                ].
 
-  Tactic Notation "induction" "finpref" ident(m) "as" ident(e) ident(f) ident(p) ident(Hp) :=
-    destruct m as [m f | m]; induction m as [|e p Hp].
+Tactic Notation "induction" "finpref" ident(m) "as" ident(e) ident(f) ident(p) ident(Hp) :=
+  destruct m as [m f | m]; induction m as [|e p Hp].
 
-  (** Prefix relation between finite prefixes and traces *)
-  (** *prefix relation *)
+(** Prefix relation between finite prefixes and traces *)
+(** *prefix relation *)
 
-  Definition prefix (m : finpref) (t : trace) : Prop :=
-    match m, t with
-    | fstop lm em, tstop lt et => em = et /\ lm = lt
-    | ftbd  lm   , tstop lt et => list_list_prefix lm lt
-    | ftbd  lm   , tsilent lt  => list_list_prefix lm lt
-    | ftbd  lm   , tstream s   => list_stream_prefix lm s
-    | _, _ => False
-    end.
+Definition prefix {E : Events} {Es : EndState}
+                  (m : @finpref E Es)
+                  (t : @trace E Es) : Prop :=
+  match m, t with
+  | fstop lm em, tstop lt et => em = et /\ lm = lt
+  | ftbd  lm   , tstop lt et => list_list_prefix lm lt
+  | ftbd  lm   , tsilent lt  => list_list_prefix lm lt
+  | ftbd  lm   , tstream s   => list_stream_prefix lm s
+  | _, _ => False
+  end.
 
-  Definition prefix_finpref (m m' : finpref) : Prop :=
+Definition prefix_finpref {E : Events} {Es : EndState}
+                          (m m' : @finpref E Es) : Prop :=
     match m, m' with
     | fstop l e, fstop l' e' => l = l' /\ e = e'
     | ftbd l, ftbd l' => l = l'
     | fstop _ _, ftbd l => False
     | ftbd l, fstop l' _ => list_list_prefix l l'
     end.
-
-End Trace.
 
 
