Diff/NonRobustSafetyCriterion.v
@@ -1,0 +1,112 @@
+From mathcomp Require Import all_ssreflect. 
+
+Set Implicit Arguments.
+Unset Printing Implicit Defensive.
+
+Require Import ClassicalExtras.
+Require Import MyNotation.
+Require Import Setoid.
+Require Import FunctionalExtensionality.
+Require Import Setoid. 
+
+Require Import Galois.
+Require Import LanguageModel.
+Require Import TraceModel.
+Require Import Properties.
+Require Import ChainModel.
+Require Import NonRobustDef.
+Require Import NonRobustSafetyDef.
+Require Import UcoPreservation. 
+
+Hypothesis prop_extensionality : forall A B : Prop, (A <-> B) -> A = B.
+
+Section SafetyCriterion.
+
+  Variable Source Target: Language.
+  Variable compilation_chain : CompilationChain Source Target.
+
+  Variable T_events S_events : Events.
+  Variable T_end S_end : EndState. 
+
+  Local Definition trace__S := @trace S_events S_end.
+  Local Definition finpref__S := @finpref S_events S_end. 
+  Local Definition trace__T := @trace T_events T_end.
+  Local Definition finpref__T := @finpref T_events T_end. 
+  
+  Local Definition prop__S := prop trace__S.
+  Local Definition Safety__S := @Safety S_events S_end. 
+  Local Definition prop__T := prop trace__T.
+  Local Definition Safety__T := @Safety T_events T_end. 
+  
+  Variable Source_Semantics : Semantics Source trace__S.
+  Variable Target_Semantics : Semantics Target trace__T. 
+
+  Local Definition sem__S := sem Source_Semantics.
+  Local Definition sem__T := sem Target_Semantics.   
+  Local Definition prg__S := prg Source.
+  Local Definition prg__T := prg Target.
+  Local Definition sat__S := sat Source_Semantics. 
+  Local Definition sat__T := sat Target_Semantics. 
+  
+  Local Definition cmp := compile_whole Source Target compilation_chain.
+
+  Local Notation "W ↓" := (cmp W) (at level 50).
+
+  Variable rel : trace__S -> trace__T -> Prop.  
+ 
+  Local Definition adjunction :=  induced_connection rel. 
+  
+  Local Definition τ' : prop__S -> prop__T := α adjunction.
+  Local Definition σ' : prop__T -> prop__S := γ adjunction.
+
+  Local Definition rel_adjunction_law : Adjunction_law τ' σ' := adjunction_law adjunction.
+
+  Local Definition Cl_τP := Cl_τP compilation_chain
+                                 Source_Semantics Target_Semantics
+                                 τ'.
+
+  
+  Local Definition σP := σP compilation_chain
+                            Source_Semantics Target_Semantics
+                            σ'.
+
+
+  Definition tilde_SC :=
+    forall W (t : trace__T) (m : finpref__T),
+      prefix m t ->  sem__T (W ↓) t ->
+      (exists t' s, rel s t' /\ prefix m t' /\ sem__S W s).
+
+  Theorem tilde_SC_σSP : tilde_SC <-> (forall W (π__T : prop__T), Safety__T π__T -> σP W π__T). 
+  Proof.
+    have G2 : Galois_snd τ' σ' by firstorder.
+    split.
+    - move => Htilde W π HSafety. setoid_rewrite contra_σP.
+      move => [t [Hsemt Hnot_t]].  
+      destruct (HSafety t Hnot_t) as [m [Hpref_m_t m_witness]]. 
+      destruct (Htilde W t m) as [t' [s [Hrel_s_t' [Hpref_m_t' Hsem_s]]]]; auto. 
+      exists s. split; auto => Hσs. 
+      have Ht0 : π t'.
+      { apply: G2; auto. now exists s. }    
+        by apply: (m_witness t').
+    - move => H_RSP W t m Hpref_m_t Hsemt.
+      have HSafetyπ : Safety__T (fun t' => ~ prefix m t').
+      { move => t'. rewrite -dne => prefix_m_t'.
+        now exists m. } 
+      move : (H_RSP W (fun t' => ~ prefix m t') HSafetyπ).
+      setoid_rewrite contra_σP => Himp. destruct Himp as [s [Hsem_s Hσ]].
+      now exists t. 
+      have : ~ (fun s': trace__S => s' = s) ⊆ (σ' (not ∘ prefix m)) by firstorder.
+      rewrite -rel_adjunction_law not_forall_ex_not. move => [t' Ht'].
+      move/not_imp: Ht' => [Ht' HHt'].
+      exists t', s. repeat (split; auto).
+      destruct Ht' as [s' [Heq Hs']]. by subst.   
+        by apply: NNPP.
+  Qed.     
+
+  Theorem tilde_SC_Cl_τTP : tilde_SC <-> (forall W (π__S : prop__S), Cl_τP W π__S).
+  Proof.
+    setoid_rewrite <- (uco_adjuncts _ _ _ safety_uco rel_adjunction_law).
+    by rewrite tilde_SC_σSP -Safety_Cl_prop. 
+  Qed.   
+  
+End SafetyCriterion. 
